annotation and step_valid of annotation

Annotation.v
@@ -17,6 +17,8 @@ Definition default_interval : interval := IInterval (Some 0) (Some 0).
 
 Definition empty : assertion := t_empty default_interval.
 
+Definition state_in_range (st : state) (s : assertion) : Prop :=
+  forall (x : id), include (s x) (st x).
 
 (* annotation :=
  * (assertion)
@@ -46,7 +48,9 @@ Definition empty : assertion := t_empty default_interval.
  *
  * While diagram :
  * (assertion)
- * while(...){
+ * while(...)
+ * (invariant)
+ * {
  *   (assertion)
  *   code
  *   (assertion)
@@ -63,7 +67,7 @@ Inductive annotation : Type :=
   | AAss : id -> aexp -> assertion -> annotation'
   | ASeq : annotation' -> annotation' -> annotation'
   | AIf : bexp -> annotation -> annotation -> assertion -> annotation'
-  | AWhile : bexp -> annotation -> assertion -> annotation'.
+  | AWhile : bexp -> assertion -> annotation -> assertion -> annotation'.
 
 Fixpoint get_com (A : annotation) : com :=
   match A with
@@ -76,15 +80,92 @@ Fixpoint get_com (A : annotation) : com :=
   | AAss x a1 _ => CAss x a1
   | ASeq A1 A2 => CSeq (get_com' A1) (get_com' A2)
   | AIf b1 A1 A2 _ => CIf b1 (get_com A1) (get_com A2)
-  | AWhile b1 A _ => CWhile b1 (get_com A)
+  | AWhile b1 _ A _ => CWhile b1 (get_com A)
   end.
 
+Definition precondition (A : annotation) : assertion :=
+  match A with
+  | APre s _ => s
+  end.
+
+Fixpoint postcondition' (A' : annotation') : assertion :=
+  match A' with
+  | ASkip s => s
+  | AAss _ _ s => s
+  | ASeq _ A2 => postcondition' A2
+  | AIf _ _ _ s => s
+  | AWhile _ _ _ s => s
+  end.
+
+Definition postcondition (A : annotation) : assertion :=
+  match A with
+  | APre _ A' => postcondition' A'
+  end.
+
+Definition valid' (s : assertion) (A' : annotation') : Prop :=
+  forall st st', get_com' A' / st \\ st' ->
+  state_in_range st s ->
+  state_in_range st' (postcondition' A').
+
+Definition valid (A : annotation) : Prop :=
+  match A with
+  | APre s A' => valid' s A'
+  end.
+
+Inductive step_valid : annotation -> Prop :=
+  | SVPre : forall s A', step_valid' s A' -> step_valid (APre s A')
+  with
+  step_valid' : assertion -> annotation' -> Prop :=
+  | SVSkip : forall s s',
+    (forall st, state_in_range st s -> state_in_range st s')
+    -> step_valid' s (ASkip s')
+  | SVAss : forall s x a s',
+    (forall st, state_in_range st s -> state_in_range (t_update st x (aeval st a)) s')
+    -> step_valid' s (AAss x a s')
+  | SVSeq : forall s A1 A2,
+    step_valid' s A1 ->
+    step_valid' (postcondition' A1) A2 ->
+    step_valid' s (ASeq A1 A2)
+  | SVIf : forall s b A1 A2 s',
+    (forall st, state_in_range st s -> beval st b = true -> state_in_range st (precondition A1)) ->
+    (forall st, state_in_range st s -> beval st b = false -> state_in_range st (precondition A2)) ->
+    step_valid A1 ->
+    step_valid A2 ->
+    (forall st, state_in_range st (postcondition A1) -> state_in_range st s') ->
+    (forall st, state_in_range st (postcondition A2) -> state_in_range st s') ->
+    step_valid' s (AIf b A1 A2 s')
+  | SVWhile : forall s b inv A s',
+    (forall st, state_in_range st s -> state_in_range st inv) ->
+    (forall st, state_in_range st inv -> beval st b = true -> state_in_range st (precondition A)) ->
+    (forall st, state_in_range st inv -> beval st b = false -> state_in_range st s') ->
+    step_valid A ->
+    (forall st, state_in_range st (postcondition A) -> state_in_range st inv) ->
+    step_valid' s (AWhile b inv A s').
+
+Scheme step_valid_ind_2 := Minimality for step_valid Sort Prop
+  with step_valid'_ind_2 := Minimality for step_valid' Sort Prop.
 
 
-
-
-
-
+Theorem step_valid_valid : forall (A : annotation),
+  step_valid A -> valid A.
+Proof.
+  apply step_valid_ind_2 with (P0 := (fun s A' => valid' s A')); intros; auto; unfold valid';
+    simpl postcondition'; simpl get_com'; intros;
+    match goal with
+    | H : _ / _ \\ _ |- _ => inversion H
+    end;
+    subst; eauto.
+  - destruct A1. eauto.
+  - destruct A2. eauto.
+  - clear dependent st'0.
+    assert (state_in_range st inv) by auto.
+    clear dependent s.
+    clear H9.
+    remember (WHILE b DO get_com A END) as c.
+    induction H5; inversion Heqc; subst.
+    + auto.
+    + apply IHceval2; auto. destruct A. eauto.
+Qed.
 
 
 
